Logic/Modal/Standard/Deduction.lean
@@ -485,4 +485,39 @@ end GL
 
 end Reducible
 
+
+section Substitution
+
+lemma GL_deduct_substitution {p : Formula α} (a : α) (q : Formula α) : 𝐆𝐋 ⊢! p → 𝐆𝐋 ⊢! (p.subst a q) := by
+  intro h;
+  induction h using Deduction.inducition_with_necOnly! with
+  | hMaxm hp =>
+    apply Deduction.maxm!;
+    rcases hp with (hAxK | hAxL);
+    . obtain ⟨p, q, rfl⟩ := hAxK; simp [Formula.subst];
+    . obtain ⟨p, q, rfl⟩ := hAxL; simp [Formula.subst];
+  | hMdp ihpq ihp =>
+    simp only [Formula.subst] at ihpq ihp;
+    exact ihpq ⨀ ihp;
+  | hNec ih =>
+    simp only [Formula.subst];
+    exact System.nec! ih;
+  | _ =>
+    simp only [Formula.subst];
+    trivial;
+
+lemma KH_deduct_substitution {p : Formula α} (a : α) (q : Formula α) : 𝐊𝐇 ⊢! p → 𝐊𝐇 ⊢! (p.subst a q) := by
+  intro h;
+  induction h using Deduction.inducition_with_necOnly! with
+  | hMaxm hp =>
+    apply Deduction.maxm!;
+    rcases hp with (hAxK | hAxH);
+    . obtain ⟨p, q, rfl⟩ := hAxK; simp [Formula.subst];
+    . obtain ⟨p, q, rfl⟩ := hAxH; simp [Formula.subst]; rfl;
+  | hMdp ihpq ihp => simp only [Formula.subst] at ihpq ihp; exact ihpq ⨀ ihp;
+  | hNec ih => simp only [Formula.subst]; exact System.nec! ih;
+  | _ => simp only [Formula.subst]; trivial;
+
+end Substitution
+
 end LO.Modal.Standard
